work in progress, revising handling of bind

pulse/src/checker/Pulse.Checker.Base.fst
@@ -250,36 +250,6 @@ let comp_st_with_post (c:comp_st) (post:term)
 let ve_unit_r g (p:term) : slprop_equiv g (tm_star p tm_emp) p = 
   VE_Trans _ _ _ _ (VE_Comm _ _ _) (VE_Unit _ _)
 
-let st_equiv_trans (#g:env) (#c0 #c1 #c2:comp) (d01:st_equiv g c0 c1) (d12:st_equiv g c1 c2)
-  : option (st_equiv g c0 c2)
-  = 
-    match d01 with
-    | ST_SLPropEquiv _f _c0 _c1 x c0_pre_typing c0_res_typing c0_post_typing eq_res_01 eq_pre_01 eq_post_01 -> (
-      let ST_SLPropEquiv _f _c1 _c2 y c1_pre_typing c1_res_typing c1_post_typing eq_res_12 eq_pre_12 eq_post_12 = d12 in
-      if x = y && eq_tm (comp_res c0) (comp_res c1)
-      then Some (
-            ST_SLPropEquiv g c0 c2 x c0_pre_typing c0_res_typing c0_post_typing
-              (RT.Rel_trans _ _ _ _ _ eq_res_01 eq_res_12)
-              (VE_Trans _ _ _ _ eq_pre_01 eq_pre_12)
-              (VE_Trans _ _ _ _ eq_post_01 eq_post_12)
-      )
-      else None
-    )
-    | ST_TotEquiv g t1 t2 u typing eq ->
-      let ST_TotEquiv _g _t1 t3 _ _ eq' = d12 in
-      let eq'' = Ghost.hide (RT.Rel_trans _ _ _ _ _ eq eq') in
-      Some (ST_TotEquiv g t1 t3 u typing eq'')
-
-let t_equiv #g #st #c (d:st_typing g st c) (#c':comp) (eq:st_equiv g c c')
-  : st_typing g st c'
-  = match d with
-    | T_Equiv _ _ _ _ d0 eq' -> (
-        match st_equiv_trans eq' eq with
-        | None -> T_Equiv _ _ _ _ d eq
-        | Some eq'' -> T_Equiv _ _ _ _ d0 eq''
-    )
-    | _ -> T_Equiv _ _ _ _ d eq
-
 let st_equiv_post (#g:env) (#t:st_term) (#c:comp_st) (d:st_typing g t c)
                   (post:term { freevars post `Set.subset` freevars (comp_post c)})
                   (veq: (x:var { fresh_wrt x g (freevars (comp_post c)) } ->
@@ -414,6 +384,10 @@ let continuation_elaborator_with_bind (#g:env) (ctxt:term)
   let framing_token : frame_for_req_in_ctxt g (tm_star ctxt pre1) pre1 = 
     (| ctxt, ctxt_typing, VE_Comm g pre1 ctxt  |)
   in
+  Pulse.Checker.Prover.Util.debug_prover g (fun _ ->
+    Printf.sprintf "Applying frame %s to computation %s\n"
+      (show ctxt)
+      (show c1));
   let (| c1, e1_typing |) =
     apply_frame ctxt_pre1_typing e1_typing framing_token in
   let (| u_of_1, pre_typing, _, _ |) =
@@ -674,7 +648,7 @@ let apply_checker_result_k (#g:env) (#ctxt:slprop) (#post_hint:post_hint_for_env
   k (Some post_hint) d
 
 #push-options "--z3rlimit_factor 4 --fuel 0 --ifuel 1"
-let checker_result_for_st_typing (#g:env) (#ctxt:slprop) (#post_hint:post_hint_opt g)
+let checker_result_for_st_typing_old (#g:env) (#ctxt:slprop) (#post_hint:post_hint_opt g)
   (d:st_typing_in_ctxt g ctxt post_hint)
   (ppname:ppname)
   : T.Tac (checker_result_t g ctxt post_hint) =
@@ -710,6 +684,51 @@ let checker_result_for_st_typing (#g:env) (#ctxt:slprop) (#post_hint:post_hint_o
   assume (~ (x `Set.mem` freevars (comp_post c)));
   let tt : universe_of _ _ _ = RU.magic () in
   (| x, g', (| comp_u c, comp_res c, tt |), (| ctxt', f x |), k |)
+
+let checker_result_for_st_typing (#g:env) (#ctxt:slprop) (#post_hint:post_hint_opt g)
+  (d:st_typing_in_ctxt g ctxt post_hint)
+  (ppname:ppname)
+: T.Tac (checker_result_t g ctxt post_hint)
+= if RU.debug_at_level (fstar_env g) "old_bind" then checker_result_for_st_typing_old d ppname
+  else 
+  let (| e1, c1, d1 |) = d in
+  let (| u_of_1, pre_typing, x, post_typing |) =
+    Metatheory.(st_comp_typing_inversion (fst <| comp_typing_inversion (st_typing_correctness d1))) in
+
+  let g' = push_binding g x ppname (comp_res c1) in
+  let ctxt' = open_term_nv (comp_post c1) (ppname, x) in
+  let k
+    : continuation_elaborator g (comp_pre c1) g' ctxt'
+    = fun post_hint st_k ->
+        let (| e2, c2, d2 |) = st_k in
+        let e2_closed = close_st_term e2 x in
+        assume (open_st_term e2_closed x == e2);
+        if x `Set.mem` freevars (comp_post c2)
+        then fail g None "Impossible: freevar clash when constructing continuation elaborator for bind, please file a bug-report"
+        else (
+          let t_typing, post_typing =
+            Pulse.Typing.Combinators.bind_res_and_post_typing g c2 x post_hint in
+          let (| ee, cc, ee_typing |) =
+            Pulse.Typing.Combinators.mk_bind
+              g (comp_pre c1)
+              e1 e2_closed c1 c2 (ppname, x)
+              d1 u_of_1
+              d2 t_typing
+              post_typing 
+              post_hint
+          in
+          (| ee, cc, ee_typing |)
+        )
+  in
+  let _ : squash (checker_res_matches_post_hint g post_hint x (comp_res c1) ctxt') =
+    match post_hint with
+    | None -> ()
+    | Some post_hint -> () in
+
+  assert (g' `env_extends` g);
+  let u_of_1_g' : universe_of _ _ _ = Pulse.Typing.Metatheory.tot_typing_weakening_standard g u_of_1 g' in
+  assert (~ (x `Set.mem` freevars (comp_post c1)));
+  (| x, g', (| _, _, u_of_1_g' |), (| ctxt', post_typing |), k |)
 #pop-options
 
 let readback_comp_res_as_comp (c:T.comp) : option comp =
