pulse/src/checker/Pulse.Checker.Bind.fst
@@ -115,6 +115,26 @@ let check_binder_typ
       ]
   end
 
+let maybe_close_post 
+  (g:env)
+  (post_hint:post_hint_opt g)
+  (ctxt:slprop)
+  (ctxt_typing:tot_typing g ctxt tm_slprop)
+  (res_ppname:ppname)
+  (r:checker_result_t g ctxt post_hint)
+: T.Tac (st_typing_in_ctxt g ctxt post_hint)
+= match post_hint with
+  | Some ph ->
+    let d = apply_checker_result_k #_ #_ #ph r res_ppname in
+    let (| _, _, dd |) = d in
+    debug_prover g (fun _ ->
+      Printf.sprintf "Derivation of continuation in bind:\n%s\n"
+        (Pulse.Typing.Printer.print_st_typing dd));
+    d
+  | _ ->
+    let (| x, g1, t, ctxt', k |) = r in
+    admit()
+
 let check_bind'
   (maybe_elaborate:bool)
   (g:env)
@@ -130,8 +150,8 @@ let check_bind'
   debug_prover g (fun _ ->
     Printf.sprintf "checking bind:\n%s\n" (P.st_term_to_string t));
 
-  if None? post_hint
-  then fail g (Some t.range) "check_bind: post hint is not set, please add an annotation";
+  // if None? post_hint
+  // then fail g (Some t.range) "check_bind: post hint is not set, please add an annotation";
 
   let Tm_Bind { binder; head=e1; body=e2 } = t.term in
   if Tm_Admit? e1.term
@@ -153,9 +173,9 @@ let check_bind'
       let g1 = reset_context g1 g in
       let d : st_typing_in_ctxt g1 ctxt' post_hint =
         let ppname = mk_ppname_no_range "_bind_c" in
-        let r =
-          check g1 ctxt' ctxt'_typing post_hint ppname (open_st_term_nv e2 (binder.binder_ppname, x)) in
-          apply_checker_result_k #_ #_ #(Some?.v post_hint) r ppname in
+        let r = check g1 ctxt' ctxt'_typing post_hint ppname (open_st_term_nv e2 (binder.binder_ppname, x)) in
+        maybe_close_post _ _ _ ctxt'_typing ppname r
+      in
       let d : st_typing_in_ctxt g ctxt post_hint = k1 post_hint d in
       checker_result_for_st_typing d res_ppname
     in
